TouhouFormal/ECL.lean
@@ -21,6 +21,7 @@ import TouhouFormal.ECL.TimedMovement
 import TouhouFormal.ECL.RandomTimedMovement
 import TouhouFormal.ECL.OrbitMovement
 import TouhouFormal.ECL.EnemyState
+import TouhouFormal.ECL.EnemyLifecycle
 import TouhouFormal.ECL.Shooting
 import TouhouFormal.ECL.TimeControl
 import TouhouFormal.ECL.BulletControl
